\documentclass{article} % For LaTeX2e
\usepackage{nips14submit_e,times}
\usepackage{amsmath}
\usepackage{amsthm}
\usepackage{amssymb}
\usepackage{mathtools}
\usepackage{hyperref}
\usepackage{url}
\usepackage{algorithm}
\usepackage[noend]{algpseudocode}
%\documentstyle[nips14submit_09,times,art10]{article} % For LaTeX 2.09

\usepackage{graphicx}
\usepackage{caption}
\usepackage{subcaption}

\def\eQb#1\eQe{\begin{eqnarray*}#1\end{eqnarray*}}
\def\eQnb#1\eQne{\begin{eqnarray}#1\end{eqnarray}}
\providecommand{\e}[1]{\ensuremath{\times 10^{#1}}}
\providecommand{\pb}[0]{\pagebreak}

\newcommand{\E}{\mathrm{E}}
\newcommand{\Var}{\mathrm{Var}}
\newcommand{\Cov}{\mathrm{Cov}}

\def\Qb#1\Qe{\begin{question}#1\end{question}}
\def\Sb#1\Se{\begin{solution}#1\end{solution}}

\newenvironment{claim}[1]{\par\noindent\underline{Claim:}\space#1}{}
\newtheoremstyle{quest}{\topsep}{\topsep}{}{}{\bfseries}{}{ }{\thmname{#1}\thmnote{ #3}.}
\theoremstyle{quest}
\newtheorem*{definition}{Definition}
\newtheorem*{theorem}{Theorem}
\newtheorem*{lemma}{Lemma}
\newtheorem*{question}{Question}
\newtheorem*{preposition}{Preposition}
\newtheorem*{exercise}{Exercise}
\newtheorem*{challengeproblem}{Challenge Problem}
\newtheorem*{solution}{Solution}
\newtheorem*{remark}{Remark}
\usepackage{verbatimbox}
\usepackage{listings}
\title{Complex Analysis I: \\
Problem Set VIII}


\author{
Youngduck Choi \\
CILVR Lab \\
New York University\\
\texttt{yc1104@nyu.edu} \\
}


% The \author macro works with any number of authors. There are two commands
% used to separate the names and addresses of multiple authors: \And and \AND.
%
% Using \And between authors leaves it to \LaTeX{} to determine where to break
% the lines. Using \AND forces a linebreak at that point. So, if \LaTeX{}
% puts 3 of 4 authors names on the first line, and the last on the second
% line, try using \AND instead of \And before the third author name.

\newcommand{\fix}{\marginpar{FIX}}
\newcommand{\new}{\marginpar{NEW}}

\nipsfinalcopy % Uncomment for camera-ready version

\begin{document}


\maketitle

\begin{abstract}
This work contains the solutions to the problem set VIII
of Complex Analysis I 2015 at Courant Institute of Mathematical Sciences.
\end{abstract}

\bigskip

\begin{question}[273-12]
\end{question}
\begin{solution}
\textbf{(a)}
As $\exp(iz^2)$ is entire, by Cauchy-Goursat theorem, we have
\eQb
\int_{C_1} \exp(iz^2) dz + \int_{C_R} \exp(iz^2)dz + \int_{C_2} 
\exp(iz^2) dz &=& 0, 
\eQe
where $C_1$ refers to the segment from $0$ to $R$, and $C_2$ refers
to the segment from $Re^{i\frac{\pi}{4}}$ to $0$. Observe that
we can parametrize points on $C_1$ as $z = x (0 \leq x \leq R)$, and
points on $C_2$ as $z = re^{i\frac{\pi}{4}} (0 \leq r \leq R)$. Therefore,
the above equality can be written as
\eQb
\int_{0}^{R} \exp(ix^2) dx &=& e^{i\frac{\pi}{4}} \int_{0}^{R} e^{-r^2} dr
- \int_{C_R} e^{iz^2} dz. \\
\eQe
Equating the real and imaginary parts separately from the above equation 
yields
\eQb
\int_{0}^{R} \cos(x^2) dx &=& \dfrac{1}{\sqrt{2}} \int_{0}^{R} e^{-r^2} dr
- \text{Re} \int_{C_R} e^{iz^2} dz, \\
\int_{0}^{R} \sin(x^2) dx &=& \dfrac{1}{\sqrt{2}} \int_{0}^{R} e^{-r^2} dr 
- \text{Im} \int_{C_R} e^{iz^z} dz.
\eQe 
\hfill $\qed$

\smallskip

\textbf{(b)}
We can parametrize the points on $C_R$ as $z = Re^{i\theta} ( 0 \leq
\theta \leq \dfrac{\pi}{4} )$. It follows that
\eQb
\int_{C_R} e^{iz^2} &=& \int_{0}^{\frac{\pi}{4}} e^{iR^2e^{i2\theta}}R
ie^{i\theta} d\theta \\
&=& 
iR \int_{0}^{\frac{\pi}{4}} e^{-R^2\sin(2\theta)} e^{iR^2\cos(2\theta)}
e^{i\theta} d\theta. \\ 
\eQe
Consequently, we have
\eQb
\left| \int_{C_R} e^{iz^2} \right| &=& 
\left| iR \int_{0}^{\frac{\pi}{4}} e^{-R^2\sin(2\theta)} 
e^{iR^2\cos(2\theta)} e^{i\theta} d\theta \right| \\ 
&\leq& 
R \int_{0}^{\frac{\pi}{4}} \left| e^{-R^2\sin(2\theta)} \right|
\left| e^{iR^2\cos(2\theta)} \right| 
\left|  e^{i\theta} \right| d\theta \\ 
&=&
R \int_{0}^{\frac{\pi}{4}} \left| e^{-R^{2}\sin(2\theta)} \right|
d\theta \\
&=&
R \int_{0}^{\frac{\pi}{4}} e^{-R^{2}\sin(2\theta)}
d\theta \\
&=& \dfrac{R}{2} 
\int_{0}^{\frac{\pi}{2}} e^{-R^2\sin(\phi)} 
d\theta , \\ 
\eQe
by change of variable $\phi = 2\theta$.
From Jordan's lemma in section 88, pg. 271, continues to 
\eQb
\left| \int_{C_R} e^{iz^2} \right| &\leq & \dfrac{R}{2}\dfrac{\pi}{2R^2} \\
&=& \dfrac{\pi}{4R}, 
\eQe
which limits $0$ as $R \to \infty$. Hence, the integral limits $0$ as
$R \to \infty$. 
\hfill $\qed$

\smallskip

\textbf{(c)}
Combining the result from (a),(b) and the given formula, we have
\eQb
\int_{0}^{\infty} \cos(x^2) dx &=& \dfrac{1}{\sqrt{2}} \int_{0}^{\infty}
e^{-x^2}dx \\
&=& \dfrac{1}{2}\sqrt{\dfrac{\pi}{2}}, \\
\int_{0}^{\infty} \sin(x^2) dx &=& \dfrac{1}{\sqrt{2}} \int_{0}^{\infty}
e^{-x^2}dx \\
&=& \dfrac{1}{2}\sqrt{\dfrac{\pi}{2}}, \\
\eQe
as desired.
\hfill $\qed$

\end{solution}

\bigskip

\begin{question}[278-1]
\end{question}
\begin{solution}
Let $f(z) = \dfrac{e^{iaz} - e^{ibz}}{z^2}$. On the indented
contour in figure 108, by Cauchy-Goursat theorem, we obtain
\eQb
\int_{L_1} f(z) dz + \int_{L_2} f(z) dz &=& -\int_{C_{\rho}} f(z) dz
- \int_{C_R} f(z) dz. \\
\eQe
Observe that on $L_1$ and $L_2$, we have the following parametric
representations:
\eQb
L_1 : z = re^{i0} = r (\rho \leq r \leq R) \> \text{ and } 
-L_2 : z = re^{i\pi} = -r (\rho \leq r \leq R).
\eQe
It follows that
\eQb
\int_{L_1} f(z) dz + \int_{L_2} f(z) dz &=& 
\int_{L_1} f(z)dz - \int_{-L_2} f(z) dz \\
&=& \int_{\rho}^{R} \dfrac{e^{iar} - e^{ibr}}{r^2} dr 
+ \int_{\rho}^{R} \dfrac{e^{-iar}- e^{-ibr}}{r^2} dr \\
&=& \int_{\rho}^{R} \dfrac{(e^{iar} + e^{-iar}) -
(e^{ibr} + e^{-ibr})}{r^2} dr \\
&=& 2\int_{\rho}^{R} \dfrac{\cos(ar) - \cos(br)}{r^2} dr.
\eQe
Now, writing the Laurent series of $f(z)$ gives
\eQb
f(z) &=& \dfrac{e^{iaz}-e^{ibz}}{z^2} \\ 
&=& \dfrac{1}{z^2}\left[ \left( 1 + \dfrac{iaz}{1!} 
+ \dfrac{(iaz)^2}{2!} ... \right) + \left( 1 + \dfrac{ibz}{1!}
+ \dfrac{(ibz)^2}{2!} ... \right) \right] \\
&=& \dfrac{i(a-b)}{z} + ... \\ 
\eQe
Therefore, we see that $z=0$ is a simple pole of $f(z)$ and the residue 
$B_0$ equals $i(a-b)$. Consequently, we obtain that
\eQb
\lim_{\rho \to 0}  \int_{C_\rho} f(z)dz = -i(a-b)\pi i = \pi(a-b).
\eQe
Observe that 
\eQb
|f(z)| \leq \dfrac{|e^{iaz}| + e^{ibz}}{|z|^2}.
\eQe
For $z$ on $C_R$, we have
\eQb
|f(z)| \leq \dfrac{2}{R^2}.
\eQe
Therefore, by $ML$ inequality, it follows that
\eQb
\left| \int_{C_R} f(z) dz \right| &\leq&
\int_{C_R} \left| f(z) \right| dz  \\ 
&\leq& \dfrac{2}{R^2}\pi R \\
&=& \dfrac{2\pi}{R}. 
\eQe
Therefore, as $R \to \infty$ $\dfrac{2\pi}{R} \to 0$, the integral
$\int_{C_R} f(z) dz$ tends to $0$ as $R \to \infty$. Consequently,
\eQb
\int_{0}^{\infty} \dfrac{\cos(ar) - \cos(br)}{r^2} dr &=& \dfrac{\pi}{2}
(b-a). 
\eQe
Setting $b=2$ and $a=0$ and using the identity $1 - \cos(2x) =
2\sin^2(x)$ , we finally obtain
\eQb
\int_{0}^{\infty} \dfrac{\sin^{2}(x)}{x^2} dx &=& \dfrac{\pi}{2}, 
\eQe
as desired. $\qed$
\end{solution}

\bigskip

\begin{question}[283-2]
\end{question}
\begin{solution}
We use the following branch as suggested:
\eQb
f(z) &=& \dfrac{z^{\frac{-1}{2}}}{z^2+1} \\
&=& \dfrac{e^{-\frac{1}{2}\log(z)}}{z^2+1} (|z| > 0, -\dfrac{\pi}{2} < 
\arg(z) < \dfrac{3\pi}{2}).
\eQe
We integrate the branch over the indented path in figure 109. 
Starting with Cauchy's residue theorem, we write
\eQb
\int_{L_1} f(z) dz + \int_{L_2} f(z) dz 
&=& 2\pi i \text{Res}_{z=i} f(z) - \int_{C_\rho} f(z) dz - \int_{C_R} f(z)dz.
\eQe
By using the parametrizations of 
\eQb
L_1 : z &=& re^{i0} = r (\rho \leq r \leq R), \\  
-L_2 : z &=& re^{i\pi} = -r (\rho \leq r \leq R),
\eQe
we obtain
\eQb
\int_{L_1} f(z) dz + \int_{L_2} f(z) dz 
&=& \int_{\rho}^{R} \dfrac{1}{\sqrt{r}(r^2+1)} dr 
- i\int_{\rho}^{R} \dfrac{1}{\sqrt{r}(r^2+1)}dr \\
&=& (1-i) \int_{\rho}^{R} \dfrac{1}{\sqrt{r}(r^2+1)} dr . 
\eQe
Observe that $z = i$ is a simple pole of $f(z)$, as it can be written that
$f(z) = \dfrac{z^{-\frac{1}{2}}}{(z+i)(z-i)}$, and $\dfrac{z^{-\frac{1}{2}}}
{(z+i)}$ is analytic and nonzero at $z = i$. Therefore, the residue at 
$z = i$ can be computed by 
\eQb
\text{Res}_{z=i} f(z) &=& \dfrac{z^{-\frac{1}{2}}}{z+i} ]_{z=i} \\
&=& \dfrac{exp(-\frac{1}{2}(\ln(1) + i\frac{\pi}{2}))}{2i}  \\
&=& \dfrac{e^{-i\frac{\pi}{4}}}{2i} \\
&=& \dfrac{1}{2i} (\dfrac{1-i}{\sqrt{2}}). 
\eQe 
For the integral terms on $C_\rho$ and $C_R$, by the ML inequality, 
we have
\eQb
\left| \int_{C_\rho} f(z) dz \right| &\leq&
\int_{C_\rho} |f(z)| dz \\
&\leq& \dfrac{\pi \rho}{\sqrt{\rho}(1-\rho^2 )} = \dfrac{\pi\sqrt{\rho}}{1-
\rho^2}, \\ 
\left| \int_{C_R} f(z) dz \right| &\leq& \int_{C_R} |f(z)| dz \\
&\leq& \dfrac{\pi \sqrt{R} }{(R^2-1)}. \\
\eQe
As $R \to \infty$ and $\rho \to 0$, we have
$\dfrac{\pi\sqrt{R}}{(R^2-1)} \to 0$, and 
$\dfrac{\pi\sqrt{\rho}}{1-\rho^2} \to 0$ respectively. Hence, it follows
that
\eQb
(1-i)\int_{0}^{\infty} \dfrac{1}{\sqrt{r}(r^2+1)} dr 
&=& \dfrac{\pi(1-i)}{\sqrt{2}},
\eQe
which can be re-written as 
\eQb
\int_{0}^{\infty} \dfrac{1}{\sqrt{r}(r^2+1)} dr 
&=& \dfrac{\pi}{\sqrt{2}},
\eQe
as desired \hfill $\qed$
\end{solution}

\bigskip

\begin{question}[283-4]
\end{question}
\begin{solution}
We use the branch $f(z) = \dfrac{\exp(\frac{1}{3}\log(z)}{(z+a)(z+b)}$,
for $|z| > 0, 0<\arg(z)<2\pi$ over the contour on section 91. 
By the reisude theorem, we have
\eQb
\int_{L_1} f(z) dz + \int_{L_2} f(z) dz + \int_{C_\rho} f(z) dz +
\int_{C_R} f(z) dz = 2\pi i (B_1 + B_2),
\eQe
where $B_1$ and $B_2$ refer to the residues from $-a$ and $-b$ respectively.
Firstly, we show that The integrals over the circular paths goes to $0$ as
follows:
\eQb
\left| \int_{C_\rho} f(z) dz \right| &\leq&
\dfrac{\rho^{\frac{1}{3}}}{(a-\rho)(b-\rho)} 2\pi \rho \\ 
&=& \dfrac{2\pi \rho^{\frac{1}{3}} \rho}{(a-\rho)(b-\rho)}. 
\eQe
As $\rho \to 0$, we see that the upper bound limits to $0$. Therefore,
the integral goes to $0$. By the same computation, we also see that
the integral over $C_R$. It follows that
\eQb
\int_{L_1} f(z) dz + \int_{L_2} f(z) dz 
= 2\pi i (B_1 + B_2).
\eQe 
The residues can be computed as follows:
\eQb
B_1 &=& \text{Res}_{z=-a} f(z) \\
&=& \dfrac{\exp(\frac{1}{3}\log(-b))}{-a+b} \\
&=& -\dfrac{\exp(\frac{1}{3}(\ln(a) + i\pi))}{a-b} \\
&=& -\dfrac{e^{i\frac{\pi}{3}a^{\frac{1}{3}}}}{a-b} \\
B_2 &=& \dfrac{e^{i\frac{\pi}{3}}b^{\frac{1}{3}}}{a-b},
\eQe
by symmetry. Using the $z = r$ parametrization on $L_1$ and $L_2$, 
we obtain
\eQb
\int_{L_1} f(z) dz + \int_{L_2} f(z) dz 
&=& \int_{\rho}^{R} (1-e^{i2\frac{\pi}{3}})
\dfrac{r^{\frac{1}{3}}}{(r+a)(r+b)} dr. 
\eQe 
Combining all the results, we obtain
\eQb
\int_{0}^{\infty} \dfrac{x^{\frac{1}{3}}}{(x+a)(x+b)} dx
&=& \dfrac{2\pi}{\sqrt{3}}\dfrac{a^{\frac{1}{3}} - b^{\frac{1}{3}}}{a-b} .
\eQe



\end{solution}

\begin{question}[283-5]
\end{question}
\begin{solution}
First, as before, we have
\eQb
\int_{0}^{\pi} \dfrac{d\theta}{(a + \cos(\theta))^2} 
&=& \dfrac{1}{2} \int_{-\pi}^{\pi} \dfrac{d\theta}{(a+\cos(\theta))^2}.
\eQe
We substitute $ \cos(\theta) = \dfrac{z + z^{-1}}{2}$, and
$d\theta = \dfrac{1}{iz}dz$ to the last integral. Then, it follows that
\eQb
\int_{-\pi}^{\pi} \dfrac{d\theta}{(a+\cos(\theta))^2} 
&=& \int_{C} \dfrac{1}{\left( a + \frac{z + z^{-1}}{2} 
\right)^2} \dfrac{1}{iz} dz \\
&=& \dfrac{4}{i}\int_{C} \dfrac{z}{(2az+z^2+1)^2} dz, 
\eQe
where $C$ denotes the contour of the unit circle.
Using the quadratic formulat, we obtain that the integrand has
a pole of order 2 at $z = -a \pm \sqrt{a^2 -1}$. As $a > 1$, we have
that $z = -a - \sqrt{a^2-1}$ is the only singular point in $C$, which
results in the residue of $\dfrac{a}{4(\sqrt{a^2-1})^3}$. Therefore,
by the residue theorem, we have
\eQb
\int_{0}^{\pi} \dfrac{d\theta}{(a + \cos(\theta))^2} &=&
\dfrac{1}{2} \dfrac{4}{i} \dfrac{2\pi i a}{4 \sqrt{a^2-1}^3} \\
&=& \dfrac{\pi a}{(\sqrt{a^2-1})^3}, 
\eQe 
as desired. \hfill $\qed$
 
\end{solution}

\bigskip

\begin{question}[287-6]
\end{question}
\begin{solution}
Observe that the following equality holds, by the linearity of integration: 
\eQb
\int_{0}^{2\pi} \dfrac{d\theta}{5 + 4\sin{\theta}} 
&=& \dfrac{1}{5} \int_{0}^{2\pi}
\dfrac{d\theta}{1+ \frac{4}{5}\sin{\theta}} \\
\eQe
From the example 1 from pg.285 in the section 92, it follows that
\eQb
\int_{0}^{2\pi} \dfrac{d\theta}{5 + 4\sin{\theta}} 
&=& \dfrac{1}{5} \int_{0}^{2\pi}
\dfrac{d\theta}{1+ \frac{4}{5}\sin{\theta}} \\
&=& \dfrac{1}{5} \dfrac{2\pi}{\sqrt{1-\frac{4}{5}^2}} \\
&=& \dfrac{1}{5} \dfrac{2\pi}{\frac{3}{5}} \\
&=& \dfrac{2}{3}\pi. 
\eQe
\hfill $\qed$
\end{solution}

\bigskip

\begin{question}[287-6]
\end{question}
\begin{solution}
As $|\sin(-\pi+\theta)| = |\sin(\theta)|$, we have $\sin^{2n}(\theta) 
= \sin^{2n}(-\pi + \theta)$, and
$\int_{0}^{\pi}\sin^{2n}(\theta) d\theta = \int_{-\pi}^{0} \sin^{2n}(\theta)
d\theta$. Hence, it follows that
\eQb
\int_{0}^{\pi} \sin^{2n}(\theta) d\theta &=& \dfrac{1}{2}\int_{C}
\sin^{2n}(\theta), \\
\eQe 
where $C$ is the positively oriented unit circle $|z| = 1$. Substituting
$\dfrac{z - z^{-1}}{2i}$ for $\sin(\theta)$, using the binomial formula,
and linearity of integration, we obtain
\eQb
\dfrac{1}{2}\int_{C} \sin^{2n}(\theta) &=& 
\dfrac{1}{2}\int_{C} {\left( \dfrac{z - z^{-1}}{2i} \right)
}^{2n} \dfrac{dz}{iz} \\
&=& \dfrac{1}{2^{2n+1}(-1)^n i} \int_{C} \dfrac{(z-z^{-1})^{2n}}{z} dz \\
&=& \dfrac{1}{2^{2n+1}(-1)^{n} i} \int_{C} \sum_{k=0}^{n} 
\binom{2n}{k}z^{k}z^{2n-k}{(-z^{-1})}^{k}z^{-1} dz \\
&=& \dfrac{1}{2^{2n+1}(-1)^{n} i} \sum_{k=0}^{n} \binom{2n}{k}
(-1)^k \int_{C} z^{2n-2k-1}dz. 
\eQe
Observe that we only get non-zero integral value for $k = n$ case,
and $\int_{C} z^{-1} dz = 2\pi i$. Therefore, it follows that
\eQb
\int_{0}^{\pi} \sin^{2n}(\theta ) d\theta &=& 
\dfrac{1}{2^{2n+1}(-1)^{n} i} \dfrac{(2n)!}{n! n!} (-1)^n 2\pi i \\
&=& \dfrac{2n!}{2^{2n} (n!)^2}\pi,
\eQe
as desired. \hfill $\qed$

\end{solution}

\bigskip

\begin{question}[293-6]
\end{question}
\begin{solution}
\textbf{(a)}
Inside the circle $|z| = 1$, write 
\eQb
f(z) = -5z^4 \> \text{ and } \> g(z) = z^6 + z^3 - 2z.
\eQe
Then, observe that when $|z| = 1$,
\eQb
|f(z)| = 5|z|^4 = 5 \> \text{ and } \> |g(z)| \leq |z|^6 + |z|^3 + 2|z| = 4.
\eQe
The conditions of Rouche's theorem are thus satisfied. Consequently, 
since $f(z)$ has 4 zeroes, counting multiplicities, inside the circle $|z| 
=1$, $f(z) + g(z)$ has 4 zeroes, inside the circle $|z| = 1$.
Therefore, the polynomial $z^6 -
5z^4 + z^3 - 2z$ has 4 zeroes, inside the circle $|z| = 1$.
\hfill $\qed$

\smallskip

\textbf{(b)}
Inside the circle $|z| = 1$, write
\eQb
f(z) = 9 \> \text{ and } \> g(z) = 2z^4 - 2z^3 + 2z^2 - 2z.
\eQe 
Then, observe that when $|z| = 1$,
\eQb
|f(z)| = 9 \> \text{ and } \> |g(z)| = 2|z|^4 + 2|z|^3 + 2|z|^2 + 2|z| = 8.
\eQe
The conditions of Rouche's theorem are thus satisfied. Consequently,
since $f(z)$ has 0 zero, counting multiplicities, inside the circle $|z| = 1$,
$f(z) + g(z)$ has 0 zero, inside the circle $|z| = 1$. Therefore, 
the polynomial $2z^4 - 2z^3 + 2z^2 - 2z + 9$ has 0 zero, inside
the circle $|z| = 1$.
\hfill $\qed$

\smallskip
\textbf{(c)} 
Inside the circle $|z| = 1$, write
\eQb
f(z) = -4z^3 \> \text{ and } \> g(z) = z^7 + z - 1. 
\eQe
Then, observe that when $|z| = 1$, 
\eQb
|f(z)| = 4|z|^3 = 4 \> \text{ and } |g(z)| \leq |z|^7 + |z| - 1 = 1.
\eQe
The conditions of Rouche's theorem are thus satisfied. Consequently,
since $f(z)$ has 3 zeroes, counting multiplicities, inside the circle
$|z| = 1$, $f(z) + g(z)$ has 3 zeroes. Therefore, the polynomial 
$z^7 - 4z^3 + z - 1$ has 3 zeroes inside the circle $|z| = 1$.
\hfill $\qed$

\end{solution}

\bigskip

\begin{question}[293-8]
\end{question}
\begin{solution}
Inside the circle $|z| = 2$, write
\eQb
f(z) = 2z^5 \> \text{ and } \> g(z) = 6z^2 + z + 1.
\eQe
Then, observe that when $|z| = 2$,
\eQb
|f(z)| = 2|z|^5 = 64 \> \text{ and } |g(z)| \leq 6|z|^2 + |z| + |1| = 8.
\eQe
The conditions of Rouche's theorem are thus satisfied. Consequently, since
$f(z)$ has 5 zeroes, counting multiplicities, inside the circle $|z| = 2$,
$f(z) + g(z)$ has 5 zeroes. On the other hand, inside the circle $|z| = 1$,
write
\eQb
f(z) = -6z^2 \> \text{ and } \> g(z) = 2z^5 + z + 1.
\eQe
Then, observe that when $|z| = 1$,
\eQb
|f(z)| = 6|z|^2 = 6 \> \text{ and } |g(z)| \leq 2|z|^5 + |z| + 1 = 4.
\eQe
The conditions of Rouche's theorem are thus satisfied. Consequently, since
$f(z)$ has 2 zeroes, counting multiplicities, inside the circle $|z| = 1 $,
$f(z) + g(z)$ has 2 zeroes. Therefore, we have shown that
in the annulus $1 \leq |z| \leq 2$, we have $5 - 2 = 3$ zeroes. 
\hfill $\qed$
\end{solution}

\end{document}

